proofs/fstar/extraction-edited/Libcrux.Kem.Kyber.Sampling.fsti
@@ -3,6 +3,30 @@ module Libcrux.Kem.Kyber.Sampling
 open Core
 open FStar.Mul
 
+val sample_from_binomial_distribution_2_ (randomness: t_Slice u8)
+    : Prims.Pure Libcrux.Kem.Kyber.Arithmetic.t_PolynomialRingElement
+      (requires (Core.Slice.impl__len randomness <: usize) =. (sz 2 *! sz 64 <: usize))
+      (ensures
+        fun result ->
+          let result:Libcrux.Kem.Kyber.Arithmetic.t_PolynomialRingElement = result in
+          Libcrux.Kem.Kyber.Arithmetic.to_spec_poly result == 
+          Spec.Kyber.sample_poly_binomial (sz 2) randomness /\
+          (forall (i:usize). i <. length result.Libcrux.Kem.Kyber.Arithmetic.f_coefficients ==>
+             (v #i32_inttype result.f_coefficients.[i] >= - 2 /\
+              v #i32_inttype result.f_coefficients.[i] <= 2)))
+
+val sample_from_binomial_distribution_3_ (randomness: t_Slice u8)
+    : Prims.Pure Libcrux.Kem.Kyber.Arithmetic.t_PolynomialRingElement
+      (requires (Core.Slice.impl__len randomness <: usize) =. (sz 3 *! sz 64 <: usize))
+      (ensures
+        fun result ->
+          let result:Libcrux.Kem.Kyber.Arithmetic.t_PolynomialRingElement = result in
+          Libcrux.Kem.Kyber.Arithmetic.to_spec_poly result == 
+          Spec.Kyber.sample_poly_binomial (sz 3) randomness /\
+         (forall (i:usize). i <. length result.Libcrux.Kem.Kyber.Arithmetic.f_coefficients ==>
+             (v #i32_inttype result.f_coefficients.[i] >= -3 /\
+              v #i32_inttype result.f_coefficients.[i] <= 3)))
+
 val sample_from_binomial_distribution (#p:Spec.Kyber.params)
     (v_ETA: usize) (randomness: t_Slice u8)
     : Pure Libcrux.Kem.Kyber.Arithmetic.t_PolynomialRingElement
